Std/Data/BinomialHeap/Lemmas.lean
@@ -8,24 +8,24 @@ import Std.Data.BinomialHeap.Basic
 namespace Std.BinomialHeap
 namespace Imp
 
-theorem Heap.findMin_val : ((s : Heap α).findMin le k res).val = s.headD le res.val :=
+theorem Heap.findMin_val {le res} : ((s : Heap α).findMin le k res).val = s.headD le res.val :=
   match s with
   | .nil => rfl
   | .cons r a c s => by rw [findMin, headD]; split <;> apply findMin_val
 
-theorem Heap.deleteMin_fst : ((s : Heap α).deleteMin le).map (·.1) = s.head? le :=
+theorem Heap.deleteMin_fst {le} : ((s : Heap α).deleteMin le).map (·.1) = s.head? le :=
   match s with
   | .nil => rfl
   | .cons r a c s => by simp only [deleteMin, findMin_val, Option.map, head?]
 
-@[simp] theorem HeapNode.WF.realSize_eq :
+@[simp] theorem HeapNode.WF.realSize_eq {le} :
     ∀ {n} {s : HeapNode α}, s.WF le a n → s.realSize + 1 = 2 ^ n
   | _, .nil, rfl => rfl
   | _, .node .., ⟨_, rfl, _, c, s⟩ => by
     rw [realSize, realSize_eq c, Nat.pow_succ, Nat.mul_succ]
     simp [Nat.add_assoc, realSize_eq s]
 
-@[simp] theorem Heap.WF.size_eq :
+@[simp] theorem Heap.WF.size_eq {le} :
     ∀ {s : Heap α}, s.WF le n → s.size = s.realSize
   | .nil, _ => rfl
   | .cons .., ⟨_, h₁, h₂⟩ => by
